Finish second eliminate_let transform
Finish Equations definition, add bool params
Prove typing, free vars, rep
Prove rewrite lemma for Why3 version

proofs/transform/eliminate_let.v
@@ -5,6 +5,73 @@ Require Import Task.
 From Equations Require Import Equations.
 Set Bullet Behavior "Strict Subproofs".
 
+(*Utilities for sublists (TODO: move?)*)
+Lemma sublist_refl {A: Type} (l: list A):
+  sublist l l.
+Proof.
+  unfold sublist. auto.
+Qed.
+
+Lemma sublist_big_union {A B: Type} 
+  (eq_dec: forall (x y: A), {x=y} + {x<>y})
+  (f: B -> list A) (l: list B) (g: B -> B):
+  Forall (fun x => sublist (f (g x)) (f x)) l ->
+  sublist (big_union eq_dec f (map g l)) (big_union eq_dec f l).
+Proof.
+  intros.
+  unfold sublist.
+  intros. simpl_set.
+  rewrite Forall_forall in H.
+  destruct H0 as [y [Hiny Hinx]].
+  rewrite in_map_iff in Hiny.
+  destruct Hiny as [z [Hy Hinz]]; subst.
+  exists z. split; auto.
+  apply H in Hinz.
+  apply Hinz; auto.
+Qed.
+
+Lemma sublist_union {A: Type} (eq_dec: forall (x y: A), {x=y}+{x<>y})
+  (l1 l2 l3 l4: list A):
+  sublist l1 l2 ->
+  sublist l3 l4 ->
+  sublist (union eq_dec l1 l3) (union eq_dec l2 l4).
+Proof.
+  unfold sublist. intros. simpl_set.
+  destruct H1; auto.
+Qed.
+
+Lemma sublist_remove {A: Type} (eq_dec: forall (x y: A), {x=y}+{x<>y})
+  v l1 l2:
+  sublist l1 l2 ->
+  sublist (remove eq_dec v l1) (remove eq_dec v l2).
+Proof.
+  unfold sublist; intros; simpl_set; destruct_all; split; auto.
+Qed.
+
+Lemma sublist_remove_all  {A: Type} (eq_dec: forall (x y: A), {x=y}+{x<>y})
+  l1 l2 l3:
+  sublist l2 l3 ->
+  sublist (remove_all eq_dec l1 l2) (remove_all eq_dec l1 l3).
+Proof.
+  unfold sublist; intros; simpl_set; destruct_all; auto.
+Qed.
+
+Ltac solve_subset :=
+  repeat match goal with
+  | |- sublist ?x ?x => apply sublist_refl
+  | |- sublist (Common.union ?eq_dec ?l1 ?l2) (Common.union ?eq_dec ?l3 ?l4) =>
+    apply sublist_union; auto
+  | |- sublist (remove ?eq_dec ?x ?l1) (remove ?eq_dec ?x ?l2) =>
+    apply sublist_remove; auto
+  | |- sublist (big_union ?eq_dec ?f (map ?g ?l)) (big_union ?eq_dec ?f ?l) =>
+    apply sublist_big_union; auto
+  | |- sublist (remove_all ?eq_dec ?l1 ?l2) (remove_all ?eq_dec ?l1 ?l3) =>
+    apply sublist_remove_all; auto
+  | H: Forall ?P (map ?f ?l) |- Forall ?Q ?l => rewrite Forall_map in H; 
+    revert H; apply Forall_impl; auto; simpl; intros
+  | |- Forall ?P ?l => rewrite Forall_forall; auto; simpl; intros; simpl
+  end.
+
 (*First version (not why3's)*)
 Section ElimLetAlt.
 
@@ -104,55 +171,6 @@ Definition elim_let_f_typed bt bf f gamma := proj_fmla
 
 (*Then prove free vars*)
 
-Lemma sublist_refl {A: Type} (l: list A):
-  sublist l l.
-Proof.
-  unfold sublist. auto.
-Qed.
-
-Lemma sublist_big_union {A B: Type} 
-  (eq_dec: forall (x y: A), {x=y} + {x<>y})
-  (f: B -> list A) (l: list B) (g: B -> B):
-  Forall (fun x => sublist (f (g x)) (f x)) l ->
-  sublist (big_union eq_dec f (map g l)) (big_union eq_dec f l).
-Proof.
-  intros.
-  unfold sublist.
-  intros. simpl_set.
-  rewrite Forall_forall in H.
-  destruct H0 as [y [Hiny Hinx]].
-  rewrite in_map_iff in Hiny.
-  destruct Hiny as [z [Hy Hinz]]; subst.
-  exists z. split; auto.
-  apply H in Hinz.
-  apply Hinz; auto.
-Qed.
-
-Lemma sublist_union {A: Type} (eq_dec: forall (x y: A), {x=y}+{x<>y})
-  (l1 l2 l3 l4: list A):
-  sublist l1 l2 ->
-  sublist l3 l4 ->
-  sublist (union eq_dec l1 l3) (union eq_dec l2 l4).
-Proof.
-  unfold sublist. intros. simpl_set.
-  destruct H1; auto.
-Qed.
-
-Lemma sublist_remove {A: Type} (eq_dec: forall (x y: A), {x=y}+{x<>y})
-  v l1 l2:
-  sublist l1 l2 ->
-  sublist (remove eq_dec v l1) (remove eq_dec v l2).
-Proof.
-  unfold sublist; intros; simpl_set; destruct_all; split; auto.
-Qed.
-
-Lemma sublist_remove_all  {A: Type} (eq_dec: forall (x y: A), {x=y}+{x<>y})
-  l1 l2 l3:
-  sublist l2 l3 ->
-  sublist (remove_all eq_dec l1 l2) (remove_all eq_dec l1 l3).
-Proof.
-  unfold sublist; intros; simpl_set; destruct_all; auto.
-Qed.
 
 (*Need sublist (not eq) because the var to sub may not
   be in the term*)
@@ -161,8 +179,7 @@ Lemma elim_let_fv bt bf (t: term) (f: formula) :
   (sublist (fmla_fv (elim_let_f bt bf f)) (fmla_fv f)).
 Proof.
   revert t f; apply term_formula_ind; simpl; intros; auto;
-  try apply sublist_refl.
-  - apply sublist_big_union; auto.
+  solve_subset. (*Only 2 nontrivial - let *)
   - destruct bt; simpl.
     + (*Need to know if var to sub appears freely in term or not*) 
       destruct (in_dec vsymbol_eq_dec v  (tm_fv (elim_let_t true bf tm2))).
@@ -173,20 +190,8 @@ Proof.
         unfold sublist. intros.
         simpl_set.
         right. split; auto.
-        intro C; subst; contradiction.
-    + apply sublist_union; auto.
-      apply sublist_remove; auto.
-  - repeat (apply sublist_union; auto).
-  - apply sublist_union; auto.
-    apply sublist_big_union; auto.
-    rewrite Forall_map in H0; revert H0. simpl.
-    apply Forall_impl; intros.
-    apply sublist_remove_all; auto.
-  - apply sublist_remove; auto.
-  - apply sublist_big_union; auto.
-  - apply sublist_remove; auto.
-  - apply sublist_union; auto.
-  - apply sublist_union; auto.
+        intro C; subst; contradiction. 
+    + solve_subset.
   - destruct bf; simpl.
     + destruct (in_dec vsymbol_eq_dec v  (fmla_fv (elim_let_f bt true f))).
       * unfold sublist. intros x.
@@ -199,12 +204,6 @@ Proof.
         intro C; subst; contradiction.
     + apply sublist_union; auto.
       apply sublist_remove; auto.
-  - repeat (apply sublist_union; auto).
-  - apply sublist_union; auto.
-    apply sublist_big_union; auto.
-    rewrite Forall_map in H0.
-    revert H0. apply Forall_impl.
-    intros. apply sublist_remove_all; auto.
 Qed.
 
 Definition elim_let_f_fv bt bf f :=
@@ -372,6 +371,16 @@ End ElimLetAlt.
     measure) only decreases if the term we substitute has no lets
     in it. Since this is a recursive call, we need the return
     type of our function to be a sigma type encoding this info.
+  6. Even this is not quite enough. For Equations to give us a 
+    good enough elimination principle, we need to take in the
+    bool parameters in the function. But they also need to be
+    Section variables, since Equations does not allow us to
+    use them in the well-founded relation otherwise (and we need
+    them; we count the number of lets that we will remove).
+    So we take in additional boolean parameters b1 and b2
+    and proofs b1 = bt and b2 = bf. We specialize these for the
+    final definition as bt bf eq_refl eq_refl, but for proofs
+    they must be generic.
 *)
 Require Import Coq.Relations.Relation_Operators.
 Section ElimLetWhy3.
@@ -517,6 +526,13 @@ Proof.
     apply IHl. lia.
 Qed.
 
+Lemma map_In_length {A B: Type} (l: list A) 
+(f: forall (x: A), In x l -> B):
+length (map_In l f) = length l.
+Proof.
+  unfold map_In; rewrite dep_map_length; auto.
+Qed.
+
 Lemma map_In_spec {A B : Type} (f : A -> B) (l : list A) :
   map_In l (fun (x : A) (_ : In x l) => f x) = map f l.
 Proof.
@@ -545,7 +561,7 @@ Proof.
     subst; auto.
 Qed.
 
-(*TODO: proof obligations about our measures*)
+(*Proof obligations about our measures*)
 Section ProofObligations.
 
 Lemma in_sum_le l x:
@@ -688,7 +704,214 @@ End ProofObligations.
 
 (*Now we can write the Equations function*)
 
-(*TODO: remove*)
+Instance elim_let_rel_wf':
+WellFounded
+        (Telescopes.tele_measure (Telescopes.tip tm_fmla) (Either term formula)
+           (fun x : tm_fmla => x) elim_let_rel).
+Proof.
+  apply elim_let_rel_wf.
+  Defined.
+
+Ltac destruct_sig :=
+  repeat match goal with
+  | |- context [(proj1_sig ?x)] => destruct x; simpl
+  end; simpl in *; try lia; auto.
+
+Ltac solve_triv_lexprod :=
+  match goal with
+  | |- slexprod nat nat lt lt (?x1, ?x2) (?x3, ?x4) =>
+    let Hle := fresh in
+    assert (Hle: x1 <= x3); [try lia|
+      let Hlt := fresh in
+      let Heq := fresh in
+      let H := fresh in
+      assert (H: x1 < x3 \/ x1 = x3) by lia;
+      destruct H as [Hlt | Heq];
+      [apply left_slex; auto | try (rewrite <- Heq); 
+        apply right_slex; auto; try lia]]
+end.
+
+Obligation Tactic := intros; try(unfold elim_let_rel, lexnat); simpl;
+try solve_triv_lexprod;
+destruct_sig.
+
+Definition tm_fmla_count_let' {x: tm_fmla} (y: tm_fmla_ty x) : nat :=
+  match x as x' return tm_fmla_ty x' -> nat with
+  | Left _ => fun t => count_let_t t
+  | Right _ => fun f => count_let_f f
+  end y.
+
+Equations elim_let_tm_fmla (x: tm_fmla) b1 b2 (Hb1: bt = b1) (Hb2: bf = b2) : 
+  { r: tm_fmla_ty x | tm_fmla_count_let' r = 0}
+  by wf x elim_let_rel :=
+(*Tlet - the interesting case*)
+elim_let_tm_fmla (Left (Tlet tm1 x tm2)) true b2 Heq1 Heq2 =>
+  (*Why we need this: not structurally recursive*)
+  elim_let_tm_fmla (Left (safe_sub_t 
+    (proj1_sig (elim_let_tm_fmla (Left tm1) true b2 Heq1 Heq2)) x tm2))
+    true b2 Heq1 Heq2
+  (*Need to retain info about bt in proof*);
+elim_let_tm_fmla (Left (Tlet tm1 x tm2)) false b2 Heq1 Heq2 =>
+  exist _ (Tlet (proj1_sig (elim_let_tm_fmla (Left tm1) false b2 Heq1 Heq2)) x 
+    (proj1_sig (elim_let_tm_fmla (Left tm2) false b2 Heq1 Heq2))) _;
+(*Other term cases*)
+elim_let_tm_fmla (Left (Tconst c)) _ _ _ _ := exist _ (Tconst c) eq_refl;
+elim_let_tm_fmla (Left (Tvar v)) _ _ _ _ := exist _ (Tvar v) eq_refl;
+elim_let_tm_fmla (Left (Tfun f tys tms)) b1 b2 Heq1 Heq2 :=
+  exist _ (Tfun f tys (map_In tms 
+    (fun x H => proj1_sig (elim_let_tm_fmla (Left x) b1 b2 Heq1 Heq2)))) _;
+elim_let_tm_fmla (Left (Tif f t1 t2)) b1 b2 Heq1 Heq2 :=
+  exist _ (Tif (proj1_sig (elim_let_tm_fmla (Right f) b1 b2 Heq1 Heq2)) 
+    (proj1_sig (elim_let_tm_fmla (Left t1) b1 b2 Heq1 Heq2))
+    (proj1_sig (elim_let_tm_fmla (Left t2) b1 b2 Heq1 Heq2))) _;
+elim_let_tm_fmla (Left (Tmatch tm ty ps)) b1 b2 Heq1 Heq2 :=
+  exist _ (Tmatch (proj1_sig (elim_let_tm_fmla (Left tm) b1 b2 Heq1 Heq2))
+    (*Coq/Equations complains without types given here*)
+    ty (@map_In (pattern * term) (pattern * term) ps 
+      (fun (x: pattern * term) H =>
+     (fst x, proj1_sig (elim_let_tm_fmla (Left (snd x)) b1 b2 Heq1 Heq2))))) _;
+elim_let_tm_fmla (Left (Teps f v)) b1 b2 Heq1 Heq2 :=
+  exist _ (Teps (proj1_sig (elim_let_tm_fmla (Right f) b1 b2 Heq1 Heq2)) v) _;
+(*Formula cases - first Flet*)
+elim_let_tm_fmla (Right (Flet t x f)) b1 true Heq1 Heq2 =>
+  (*Why we need this: not structurally recursive*)
+  elim_let_tm_fmla (Right (safe_sub_f 
+    (proj1_sig (elim_let_tm_fmla (Left t) b1 true Heq1 Heq2)) x f))
+    b1 true Heq1 Heq2;
+elim_let_tm_fmla (Right (Flet t x f)) b1 false Heq1 Heq2 =>
+  exist _ (Flet (proj1_sig (elim_let_tm_fmla (Left t) b1 false Heq1 Heq2)) x 
+    (proj1_sig (elim_let_tm_fmla (Right f) b1 false Heq1 Heq2))) _;
+elim_let_tm_fmla (Right (Fpred p tys tms)) b1 b2 Heq1 Heq2 :=
+  exist _ (Fpred p tys (map_In tms 
+  (fun x H => proj1_sig (elim_let_tm_fmla (Left x) b1 b2 Heq1 Heq2)))) _;
+elim_let_tm_fmla (Right (Fquant q v f)) b1 b2 Heq1 Heq2 :=
+  exist _ (Fquant q v (proj1_sig (elim_let_tm_fmla (Right f) b1 b2 Heq1 Heq2))) _;
+elim_let_tm_fmla (Right (Feq ty t1 t2)) b1 b2 Heq1 Heq2 :=
+  exist _ (Feq ty (proj1_sig (elim_let_tm_fmla (Left t1) b1 b2 Heq1 Heq2)) 
+    (proj1_sig (elim_let_tm_fmla (Left t2) b1 b2 Heq1 Heq2))) _;
+elim_let_tm_fmla (Right (Fbinop b f1 f2)) b1 b2 Heq1 Heq2 :=
+  exist _ (Fbinop b (proj1_sig (elim_let_tm_fmla (Right f1) b1 b2 Heq1 Heq2)) 
+    (proj1_sig (elim_let_tm_fmla (Right f2) b1 b2 Heq1 Heq2))) _;
+elim_let_tm_fmla (Right (Fnot f)) b1 b2 Heq1 Heq2 :=
+  exist _ (Fnot (proj1_sig (elim_let_tm_fmla (Right f) b1 b2 Heq1 Heq2))) _;
+elim_let_tm_fmla (Right Ftrue) _ _ _ _ := exist _ Ftrue eq_refl;
+elim_let_tm_fmla (Right Ffalse) _ _ _ _ := exist _ Ffalse eq_refl;
+elim_let_tm_fmla (Right (Fif f1 f2 f3)) b1 b2 Heq1 Heq2 :=
+  exist _ (Fif (proj1_sig (elim_let_tm_fmla (Right f1) b1 b2 Heq1 Heq2)) 
+    (proj1_sig (elim_let_tm_fmla (Right f2) b1 b2 Heq1 Heq2))
+    (proj1_sig (elim_let_tm_fmla (Right f3) b1 b2 Heq1 Heq2))) _;
+elim_let_tm_fmla (Right (Fmatch tm ty ps)) b1 b2 Heq1 Heq2 :=
+  exist _ (Fmatch (proj1_sig (elim_let_tm_fmla (Left tm) b1 b2 Heq1 Heq2))
+  (*Coq/Equations complains without types given here*)
+  ty (@map_In (pattern * formula) (pattern * formula) ps 
+    (fun x H =>
+    (fst x, proj1_sig (elim_let_tm_fmla (Right (snd x)) b1 b2 Heq1 Heq2))))) _.
+Next Obligation.
+(*Because of [map_In], we have the hypothesis we need*)
+- apply in_sum_le; rewrite in_map_iff. exists x; auto.
+- apply Arith_prebase.le_lt_n_Sm_stt.
+  apply in_sum_le.
+  rewrite in_map_iff; exists x; auto.
+Defined.
+Next Obligation.
+(*Tfun number of lets*)
+apply sum_0.
+rewrite Forall_forall. intros.
+rewrite in_map_iff in H.
+destruct H as [t [Hx Hint]]; subst.
+rewrite in_map_In_iff in Hint.
+destruct Hint as [x [Hinx Ht]]; subst.
+destruct_sig.
+Defined.
+Next Obligation.
+(*Hard one: the non-structurally-recursive let call*)
+- subst. rewrite Heq1. (*We need info about bt*)
+  (*Here, we need the info from the dependent type*)
+  rewrite count_let_safe_sub_t; try lia.
+- subst. rewrite Heq1 in H, H1.
+  rewrite count_let_safe_sub_t in H, H1; auto. lia.
+Defined.
+Next Obligation.
+(*bt=false number of lets*)
+subst. rewrite Heq1. lia. 
+Defined.
+Next Obligation.
+(*Tmatch termination*)
+- eapply Nat.le_trans; [| apply Nat.le_add_l].
+  apply in_sum_le. rewrite in_map_iff. exists x; auto.
+- apply Arith_prebase.le_lt_n_Sm_stt.
+  eapply Nat.le_trans; [| apply Nat.le_add_l].
+  apply in_sum_le. rewrite in_map_iff. exists x; auto.
+Defined.
+Next Obligation.
+(*Tmatch number of lets*)
+rewrite e; simpl.
+apply sum_0.
+rewrite Forall_forall; intros.
+rewrite in_map_iff in H.
+destruct H as [p [Hp Hinx]]; subst.
+rewrite in_map_In_iff in Hinx.
+destruct Hinx as [p1 [Hin Hp]]; subst; simpl.
+destruct_sig.
+Defined.
+Next Obligation.
+(*Fpred termination*)
+- apply in_sum_le; rewrite in_map_iff. exists x; auto.
+- apply Arith_prebase.le_lt_n_Sm_stt.
+  apply in_sum_le.
+  rewrite in_map_iff; exists x; auto.
+Defined.
+Next Obligation.
+(*Fpred number of lets*)
+apply sum_0.
+rewrite Forall_forall. intros.
+rewrite in_map_iff in H.
+destruct H as [t [Hx Hint]]; subst.
+rewrite in_map_In_iff in Hint.
+destruct Hint as [x [Hinx Ht]]; subst.
+destruct_sig.
+Defined.
+Next Obligation.
+(* non-structurally-recursive let call*)
+- subst. rewrite Heq2. (*We need info about bt*)
+  (*Here, we need the info from the dependent type*)
+  rewrite count_let_safe_sub_f; lia.
+- subst. rewrite Heq2 in H, H1.
+  rewrite count_let_safe_sub_f in H, H1; lia.
+Defined.
+Next Obligation.
+(*bt=false number of lets*)
+subst. rewrite Heq2; lia.
+Defined.
+Next Obligation.
+(*Fmatch termination*)
+- eapply Nat.le_trans; [| apply Nat.le_add_l].
+  apply in_sum_le. rewrite in_map_iff. exists x; auto.
+- apply Arith_prebase.le_lt_n_Sm_stt.
+  eapply Nat.le_trans; [| apply Nat.le_add_l].
+  apply in_sum_le. rewrite in_map_iff. exists x; auto.
+Defined.
+Next Obligation.
+(*Fmatch number of lets*)
+rewrite e; simpl.
+apply sum_0.
+rewrite Forall_forall; intros.
+rewrite in_map_iff in H.
+destruct H as [p [Hp Hinx]]; subst.
+rewrite in_map_In_iff in Hinx.
+destruct Hinx as [p1 [Hin Hp]]; subst; simpl.
+destruct_sig.
+Defined.
+
+(*Now our function is defined. We can define the term and
+  formula versions and show that underneath all of the dependent
+  types, we have the functions we expect*)
+Section RewriteLemma.
+
+(*First, as why3 does, we include a mapping function
+  over terms and formulas for the recursive cases*)
+(*NOTE: we cannot use this in the Equations definition;
+  we get unsolvable proof obligations*)
 
 (*Not binding or type safe*)
 Definition t_map (f1: term -> term) (f2: formula -> formula) 
@@ -718,145 +941,402 @@ Definition f_map (f1: term -> term) (f2: formula -> formula)
   | _ => f
   end.
 
-Instance elim_let_rel_wf':
-WellFounded
-        (Telescopes.tele_measure (Telescopes.tip tm_fmla) (Either term formula)
-           (fun x : tm_fmla => x) elim_let_rel).
+(*Do in 2 pieces*)
+Definition elim_let_tm_aux b1 b2 Heq1 Heq2 (t: term) : term :=
+  proj1_sig (elim_let_tm_fmla (Left t) b1 b2 Heq1 Heq2).
+Definition elim_let_fmla_aux b1 b2 Heq1 Heq2 (f: formula)  : formula :=
+  proj1_sig (elim_let_tm_fmla (Right f) b1 b2 Heq1 Heq2).
+
+(*The actual functions*)
+Definition elim_let_tm (t: term) : term :=
+  elim_let_tm_aux bt bf eq_refl eq_refl t.
+Definition elim_let_fmla (f: formula) : formula :=
+  elim_let_fmla_aux bt bf eq_refl eq_refl f.
+
+Lemma elim_let_tm_eq_aux (t: term) b1 b2 Heq1 Heq2 :
+  elim_let_tm_aux b1 b2 Heq1 Heq2 t =
+  match t with
+  | Tlet t1 v t2 =>
+    let t1' := elim_let_tm_aux b1 b2 Heq1 Heq2 t1 in
+    if bt then
+    elim_let_tm_aux b1 b2 Heq1 Heq2 (safe_sub_t t1' v t2)
+    else Tlet t1' v (elim_let_tm_aux b1 b2 Heq1 Heq2 t2)
+  | _ => t_map (elim_let_tm_aux b1 b2 Heq1 Heq2) 
+    (elim_let_fmla_aux b1 b2 Heq1 Heq2) t
+  end.
 Proof.
-  apply elim_let_rel_wf.
-  Defined.
+  unfold elim_let_tm_aux; destruct t; simpl; auto.
+  - rewrite elim_let_tm_fmla_equation_1; reflexivity.
+  - rewrite elim_let_tm_fmla_equation_2; reflexivity.
+  - rewrite elim_let_tm_fmla_equation_3; reflexivity.
+  - (*We need aux so we can destruct without dependent type issues*) 
+    destruct b1; subst; simpl.
+    + rewrite Heq1 at 1.
+      rewrite elim_let_tm_fmla_equation_4; reflexivity.
+    + rewrite Heq1 at 1.
+      rewrite elim_let_tm_fmla_equation_5; reflexivity.
+  - rewrite elim_let_tm_fmla_equation_6; reflexivity.
+  - rewrite elim_let_tm_fmla_equation_7; simpl.
+    f_equal. apply map_In_spec.
+  - rewrite elim_let_tm_fmla_equation_8; reflexivity.
+Qed.
 
-Ltac destruct_sig :=
-  repeat match goal with
-  | |- context [(proj1_sig ?x)] => destruct x; simpl
-  end; simpl in *; try lia; auto.
+(*The theorem we want: 
+  the definition in why3/src/transform/eliminate_let.ml*)
+Theorem elim_let_tm_eq (t: term) :
+elim_let_tm t =
+match t with
+| Tlet t1 v t2 =>
+  let t1' := elim_let_tm t1 in
+  if bt then
+  elim_let_tm (safe_sub_t t1' v t2)
+  else Tlet t1' v (elim_let_tm t2)
+| _ => t_map elim_let_tm elim_let_fmla t
+end.
+Proof.
+  apply elim_let_tm_eq_aux.
+Qed.
 
-Obligation Tactic := intros; try(unfold elim_let_rel, lexnat); simpl;
-destruct_sig.
+Lemma elim_let_fmla_eq_aux (f: formula) b1 b2 Heq1 Heq2 :
+  elim_let_fmla_aux b1 b2 Heq1 Heq2 f =
+  match f with
+  | Flet t v f =>
+    let t1' := elim_let_tm_aux b1 b2 Heq1 Heq2 t in
+    if bf then
+    elim_let_fmla_aux b1 b2 Heq1 Heq2 (safe_sub_f t1' v f)
+    else Flet t1' v (elim_let_fmla_aux b1 b2 Heq1 Heq2 f)
+  | _ => f_map (elim_let_tm_aux b1 b2 Heq1 Heq2) 
+    (elim_let_fmla_aux b1 b2 Heq1 Heq2) f
+  end.
+Proof.
+  unfold elim_let_fmla_aux; destruct f; simpl; auto.
+  - rewrite elim_let_tm_fmla_equation_9; simpl; 
+    rewrite map_In_spec; reflexivity.
+  - rewrite elim_let_tm_fmla_equation_10; reflexivity.
+  - rewrite elim_let_tm_fmla_equation_11; reflexivity.
+  - rewrite elim_let_tm_fmla_equation_12; reflexivity.
+  - rewrite elim_let_tm_fmla_equation_13; reflexivity.
+  - rewrite elim_let_tm_fmla_equation_14; reflexivity.
+  - rewrite elim_let_tm_fmla_equation_15; reflexivity.
+  - (*We need aux so we can destruct without dependent type issues*) 
+    destruct b2; subst; simpl.
+    + rewrite Heq2 at 1.
+      rewrite elim_let_tm_fmla_equation_16; reflexivity.
+    + rewrite Heq2 at 1.
+      rewrite elim_let_tm_fmla_equation_17; reflexivity.
+  - rewrite elim_let_tm_fmla_equation_18; reflexivity.
+  - rewrite elim_let_tm_fmla_equation_19; simpl.
+    f_equal. apply map_In_spec.
+Qed.
 
-Definition tm_fmla_count_let' {x: tm_fmla} (y: tm_fmla_ty x) : nat :=
-  match x as x' return tm_fmla_ty x' -> nat with
-  | Left _ => fun t => count_let_t t
-  | Right _ => fun f => count_let_f f
+Lemma elim_let_fmla_eq (f: formula) :
+  elim_let_fmla f =
+  match f with
+  | Flet t v f =>
+    let t' := elim_let_tm t in
+    if bf then
+    elim_let_fmla (safe_sub_f t' v f)
+    else Flet t' v (elim_let_fmla f)
+  | _ => f_map elim_let_tm elim_let_fmla f
+  end.
+Proof.
+  apply elim_let_fmla_eq_aux.
+Qed.
+
+End RewriteLemma.
+
+(*Now we have to prove soundness. This is more difficult because 
+  we can't use structural induction; we use the induction principle
+  generated by Equations. But this means that our theorem
+  statements must be a bit awkward*)
+
+(*First, typing*)
+Section Typing.
+Variable gamma: context.
+
+(*We need a separate definition for our prop*)
+Definition elim_let_tm_fmla_ty (x: tm_fmla) (y: tm_fmla_ty x) : Prop :=
+  match x as x' return tm_fmla_ty x' -> Prop with
+  | Left t1 => fun t2 => 
+    forall ty, term_has_type gamma t1 ty -> term_has_type gamma t2 ty
+  | Right f1 => fun f2 =>
+    formula_typed gamma f1 -> formula_typed gamma f2
   end y.
 
+Lemma elim_let_tm_fmla_typed (x: tm_fmla) b1 b2 Heq1 Heq2:
+  elim_let_tm_fmla_ty x (proj1_sig (elim_let_tm_fmla x b1 b2 Heq1 Heq2)).
+Proof.
+  apply elim_let_tm_fmla_elim; intros; simpl; intros; auto; simpl in *.
+  - inversion H1; subst; auto.
+    rewrite map_In_spec. constructor; auto;
+    [rewrite map_length; auto|].
+    assert (length tms = length (map (ty_subst (s_params f) tys) (s_args f)))
+      by (rewrite map_length; auto).
+    generalize dependent (map (ty_subst (s_params f) tys) (s_args f)).
+    clear -H.
+    induction tms; simpl; intros; auto.
+    destruct l; inversion H2. inversion H12; subst; simpl in H. 
+    constructor; auto.
+    apply H; auto.
+  - (*Without the b1 b2 Heq1 Heq2, Equations does not give us
+    a good enough IH here - don't know about [safe_sub]*)
+    apply H0. destruct x0 as [x1 x2].
+    inversion H1; subst; simpl in *. 
+    apply safe_sub_t_typed; auto.
+  - inversion H2; subst. constructor; auto.
+  - inversion H3; subst.
+    constructor; auto.
+  - rewrite map_In_spec. 
+    inversion H2; subst. constructor; auto; [| |rewrite null_map; auto];
+    intros p; rewrite in_map_iff; 
+    intros [p1 [Hp Hinp1]]; subst; simpl; auto.
+  - inversion H1; subst. constructor; auto.
+  - inversion H1; subst. rewrite map_In_spec; constructor; auto;
+    try rewrite map_length; auto.
+    assert (length tms = length (map (ty_subst (s_params p) tys) (s_args p)))
+      by (rewrite map_length; auto).
+    generalize dependent (map (ty_subst (s_params p) tys) (s_args p)).
+    clear -H.
+    induction tms; simpl; intros; auto.
+    destruct l; inversion H2. inversion H10; subst; simpl in H. 
+    constructor; auto.
+    apply H; auto.
+  - inversion H1; subst. constructor; auto.
+  - inversion H2; subst. constructor; auto.
+  - inversion H2; subst. constructor; auto.
+  - inversion H1; subst. constructor; auto.
+  - inversion H1; subst. apply H0. destruct x0 as [x1 x2]. 
+    apply safe_sub_f_typed; auto.
+  - inversion H2; subst. constructor; auto.
+  - inversion H3; subst. constructor; auto.
+  - rewrite map_In_spec. 
+    inversion H2; subst. constructor; auto; [| |rewrite null_map; auto];
+    intros p; rewrite in_map_iff; 
+    intros [p1 [Hp Hinp1]]; subst; simpl; auto.
+Qed.
+
+(*And our corollaries*)
+Lemma elim_let_tm_typed (t: term) (ty: vty):
+  term_has_type gamma t ty ->
+  term_has_type gamma (elim_let_tm t) ty.
+Proof.
+  intros.
+  apply (elim_let_tm_fmla_typed (Left t) bt bf eq_refl eq_refl);
+  auto.
+Qed.
+
+Lemma elim_let_fmla_typed (f: formula):
+  formula_typed gamma f ->
+  formula_typed gamma (elim_let_fmla f).
+Proof.
+  intros.
+  apply (elim_let_tm_fmla_typed (Right f) bt bf eq_refl eq_refl);
+  auto.
+Qed.
+
+End Typing.
+
+(*Part 2: free vars*)
+Section FreeVars.
 
 
-Equations elim_let_tm_fmla (x: tm_fmla) : 
-  { r: tm_fmla_ty x | tm_fmla_count_let' r = 0}
-  by wf x elim_let_rel :=
-elim_let_tm_fmla (Left (Tlet tm1 x tm2)) =>
-  let t1 := proj1_sig (elim_let_tm_fmla (Left tm1)) in
-  (*Need to retain info about bt in proof*)
-  match bt as b return bt = b -> 
-  {r : tm_fmla_ty (Left (Tlet tm1 x tm2)) | tm_fmla_count_let' r = 0} with
-  (*Why we need this: not structurally recursive*)
-  | true => fun Hb => 
-     elim_let_tm_fmla (Left (safe_sub_t t1 x tm2))
-  | false => fun Hb => 
-    exist _ (Tlet t1 x (proj1_sig (elim_let_tm_fmla (Left tm2)))) _
-  end eq_refl ;
-elim_let_tm_fmla (Left (Tconst c)) := exist _ (Tconst c) eq_refl;
-elim_let_tm_fmla (Left (Tvar v)) := exist _ (Tvar v) eq_refl;
-elim_let_tm_fmla (Left (Tfun f tys tms)) :=
-  exist _ (Tfun f tys (map_In tms 
-    (fun x H => proj1_sig (elim_let_tm_fmla (Left x))))) _;
-elim_let_tm_fmla (Left (Tif f t1 t2)) :=
-  exist _ (Tif (proj1_sig (elim_let_tm_fmla (Right f))) 
-    (proj1_sig (elim_let_tm_fmla (Left t1)))
-    (proj1_sig (elim_let_tm_fmla (Left t2)))) _;
-elim_let_tm_fmla (Left t) := exist _ (t_map 
-  (fun x => proj1_sig (elim_let_tm_fmla (Left x)))
-  (fun x => proj1_sig (elim_let_tm_fmla (Right x))) t) _;
-elim_let_tm_fmla (Right (Flet t x f)) =>
-  let t1 := proj1_sig (elim_let_tm_fmla (Left t)) in
-  (*Need to retain info about bt in proof*)
-  match bf as b return bf = b -> 
-  {r : tm_fmla_ty (Right (Flet t x f)) | tm_fmla_count_let' r = 0} with
-  (*Why we need this: not structurally recursive*)
-  | true => fun Hb => 
-    elim_let_tm_fmla (Right (safe_sub_f t1 x f))
-  | false => fun Hb => 
-    exist _ (Flet t1 x (proj1_sig (elim_let_tm_fmla (Right f)))) _
-  end eq_refl ;
-elim_let_tm_fmla (Right f) := exist _ (f_map 
-(fun x => proj1_sig (elim_let_tm_fmla (Left x)))
-(fun x => proj1_sig (elim_let_tm_fmla (Right x))) f) _.
-Next Obligation.
-(*Tfun termination*)
-(*Because of [map_In], we have the hypothesis we need*)
-assert (count_let_t x <= sum (map count_let_t tms)). {
-  apply in_sum_le; rewrite in_map_iff. exists x; auto.
-}
-apply Lt.le_lt_or_eq_stt in H0.
-destruct H0.
-- apply left_slex; auto.
-- rewrite H0. apply right_slex.
-  apply Arith_prebase.le_lt_n_Sm_stt.
-  apply in_sum_le.
-  rewrite in_map_iff; exists x; auto.
-Defined.
-Next Obligation.
-(*Tfun number of lets*)
-apply sum_0.
-rewrite Forall_forall. intros.
-rewrite in_map_iff in H.
-destruct H as [t [Hx Hint]]; subst.
-rewrite in_map_In_iff in Hint.
-destruct Hint as [x [Hinx Ht]]; subst.
-destruct_sig.
-Defined.
-Next Obligation.
-(*First let (t1) termination*)
-destruct bt; simpl.
-- apply left_slex. (*TODO: avoid lia maybe*) lia.
-- destruct (count_let_t tm2).
-  + rewrite !Nat.add_0_r. apply right_slex.
-    lia.
-  + apply left_slex; lia.
-Defined.
-Next Obligation.
-(*Hard one: the non-structurally-recursive let call*)
-rewrite Hb. (*We need info about bt*)
-(*Here, we need the info from the dependent type*)
-rewrite count_let_safe_sub_t.
-- apply left_slex. lia.
-- subst t1. simpl.
-  destruct ((elim_let_tm_fmla (Left tm1) 
-    (elim_let_tm_fmla_obligations_obligation_3 tm1 x tm2)));
-  simpl; auto.
-Defined.
-Next Obligation.
-(*The other let case (bt false)*)
-rewrite Hb.
-destruct (count_let_t tm1).
-- simpl. apply right_slex. lia.
-- apply left_slex; lia.
-Defined.
-Next Obligation.
-(*bt=false number of lets*)
-rewrite Hb at 1.
-rewrite Nat.add_0_r.
-subst t1; simpl.
-destruct_sig.
-Defined.
-Next Obligation.
-(*Termination for Tif - case 1*)
-rewrite <- Nat.add_assoc.
-destruct (count_let_t t1 + count_let_t t2);
-[rewrite Nat.add_0_r; apply right_slex| apply left_slex]; lia.
-Defined.
-Next Obligation.
-(*Tif termination 2*)
-rewrite (Nat.add_comm _ (count_let_t t1)), <- Nat.add_assoc.
-destruct (count_let_f f + count_let_t t2);
-[rewrite Nat.add_0_r; apply right_slex | apply left_slex]; lia.
-Defined.
-Next Obligation.
-(*Tif termination 3*)
-destruct (count_let_f f + count_let_t t1);
-[apply right_slex | apply left_slex]; lia.
-Defined.
-Next Obligation.
-(*Tmatch termination 1*)
-(*TODO: fix program, no map*)
+(*We need a separate definition for our prop*)
+Definition elim_let_tm_fmla_fv_sublist (x: tm_fmla) (y: tm_fmla_ty x) : Prop :=
+  match x as x' return tm_fmla_ty x' -> Prop with
+  | Left t1 => fun t2 => 
+    sublist (tm_fv t2) (tm_fv t1)
+  | Right f1 => fun f2 =>
+    sublist (fmla_fv f2) (fmla_fv f1)
+  end y.
+
+Lemma elim_let_tm_fmla_fv (x: tm_fmla) b1 b2 Heq1 Heq2:
+elim_let_tm_fmla_fv_sublist x (proj1_sig (elim_let_tm_fmla x b1 b2 Heq1 Heq2)).
+Proof.
+  apply elim_let_tm_fmla_elim; intros; simpl; intros; auto; simpl in *;
+  try (rewrite map_In_spec); solve_subset;
+  try solve[ rewrite Forall_forall; auto]. 
+  (*Only 2 nontrivial goals - let*) 
+  - eapply sublist_trans. apply H0. unfold sublist. intros.
+    destruct (in_dec vsymbol_eq_dec x0 (tm_fv tm2)).
+    + rewrite safe_sub_t_fv in H1; auto.
+      simpl_set. destruct H1; auto.
+    + rewrite safe_sub_t_notin in H1; auto.
+      simpl_set. right; split; auto. intro C; subst; contradiction.
+  - eapply sublist_trans. apply H0. unfold sublist. intros.
+    destruct (in_dec vsymbol_eq_dec x0 (fmla_fv f)).
+    + rewrite safe_sub_f_fv in H1; auto.
+      simpl_set. destruct H1; auto.
+    + rewrite safe_sub_f_notin in H1; auto.
+      simpl_set. right; split; auto. intro C; subst; contradiction.
+Qed.
+
+(*Corollary:*)
+Lemma elim_let_fmla_fv (f: formula):
+  sublist (fmla_fv (elim_let_fmla f)) (fmla_fv f).
+Proof.
+  apply (elim_let_tm_fmla_fv (Right f) bt bf eq_refl eq_refl);
+  auto.
+Qed.
+
+End FreeVars.
+
+(*Last piece: preserves semantics*)
+Section Rep.
+
+Context {gamma: context} (gamma_valid: valid_context gamma) 
+  (pd: pi_dom) (vt: val_typevar) (pf: pi_funpred gamma_valid pd).
+
+Definition elim_let_tm_fmla_rep_eq (x: tm_fmla) (y: tm_fmla_ty x) : Prop :=
+  match x as x' return tm_fmla_ty x' -> Prop with
+  | Left t1 => fun t2 => 
+    forall vv ty (Hty1: term_has_type gamma t1 ty) 
+      (Hty2: term_has_type gamma t2 ty),
+    term_rep gamma_valid pd vt pf vv t2 ty Hty2 =
+    term_rep gamma_valid pd vt pf vv t1 ty Hty1
+  | Right f1 => fun f2 =>
+    forall vv (Hty1: formula_typed gamma f1)
+      (Hty2: formula_typed gamma f2),
+    formula_rep gamma_valid pd vt pf vv f2 Hty2 =
+    formula_rep gamma_valid pd vt pf vv f1 Hty1
+  end y.
+
+Lemma elim_let_tm_fmla_rep (x: tm_fmla) b1 b2 Heq1 Heq2:
+elim_let_tm_fmla_rep_eq x (proj1_sig (elim_let_tm_fmla x b1 b2 Heq1 Heq2)).
+Proof.
+  apply elim_let_tm_fmla_elim; intros; simpl; intros; auto; simpl in *;
+  try apply term_rep_irrel; simpl_rep_full.
+  - (*TODO: fix*)
+    assert (ty_fun_ind_ret Hty2 = ty_fun_ind_ret Hty1).
+      apply UIP_dec. apply vty_eq_dec.
+    rewrite H1. f_equal. f_equal. apply UIP_dec. apply sort_eq_dec.
+    f_equal. clear H1. revert Hty2.
+    rewrite map_In_spec; intros.
+    apply get_arg_list_ext; rewrite map_length; auto.
+    intros.
+    revert Hty0.
+    rewrite map_nth_inbound with(d2:=tm_d); auto; intros.
+    apply H. apply nth_In; auto.
+  - (*Tlet case 1*)
+    inversion Hty1; subst.
+    destruct x0 as [x1 x2]. erewrite H0.  erewrite safe_sub_t_rep.
+    erewrite H. reflexivity.
+    Unshelve.
+    apply safe_sub_t_typed; auto.
+    all: apply (elim_let_tm_fmla_typed gamma (Left tm1)); auto.
+  - (*Tlet case 2*)
+    erewrite H, H0. reflexivity.
+  - (*Tif*) erewrite H, H0, H1; reflexivity.
+  - (*Tmatch*)
+    revert Hty2. clear H1.
+    rewrite !map_In_spec; intros.
+    iter_match_gen Hty1 Htm1 Hpat1 Hty1.
+    iter_match_gen Hty2 Htm2 Hpat2 Hty2.
+    induction ps; simpl; intros; auto.
+    simpl in *. destruct a as [p1 t1];
+    simpl in *.
+    rewrite H with(Hty1:=Hty1) at 1.
+    rewrite match_val_single_irrel with (Hval2:=(Forall_inv Hpat1)).
+    simpl.
+    case_match_goal; auto.
+    apply (H0 (p1, t1)); auto.
+  - f_equal. apply functional_extensionality_dep; intros.
+    assert ((proj2' (ty_eps_inv Hty2)) = (proj2' (ty_eps_inv Hty1))). {
+      apply UIP_dec. apply vty_eq_dec.
+    }
+    erewrite H, H1. reflexivity.
+  - f_equal. revert Hty2. 
+    rewrite map_In_spec; intros.
+    apply get_arg_list_ext; rewrite map_length; auto.
+    intros.
+    revert Hty0.
+    rewrite map_nth_inbound with(d2:=tm_d); auto; intros.
+    apply H. apply nth_In; auto.
+  - destruct q; simpl_rep_full; apply all_dec_eq; split;
+    [intros Hd d | intros Hd d| intros [d Hd]; exists d |
+    intros [d Hd]; exists d];
+    try (erewrite H; apply Hd);
+    erewrite <- H; apply Hd.
+  - erewrite H, H0; reflexivity.
+  - erewrite H, H0; reflexivity.
+  - f_equal. apply H.
+  - (*Flet case 1*)
+    inversion Hty1; subst.
+    destruct x0 as [x1 x2]. erewrite H0.  erewrite safe_sub_f_rep.
+    erewrite H. reflexivity.
+    Unshelve.
+    apply safe_sub_f_typed; auto.
+    all: apply (elim_let_tm_fmla_typed gamma (Left t)); auto.
+  - (*Flet case 2*)
+    erewrite H, H0. reflexivity.
+  - (*Fif*) erewrite H, H0, H1; reflexivity.
+  - (*Fmatch*)
+    revert Hty2. clear H1.
+    rewrite !map_In_spec; intros.
+    iter_match_gen Hty1 Htm1 Hpat1 Hty1.
+    iter_match_gen Hty2 Htm2 Hpat2 Hty2.
+    induction ps; simpl; intros; auto.
+    simpl in *. destruct a as [p1 t1];
+    simpl in *.
+    rewrite H with(Hty1:=Hty1) at 1.
+    rewrite match_val_single_irrel with (Hval2:=(Forall_inv Hpat1)).
+    simpl.
+    case_match_goal; auto.
+    apply (H0 (p1, t1)); auto.
+Qed.
+
+(*And the corollary:*)
+Lemma elim_let_fmla_rep vv (f: formula) :
+  forall (Hty1: formula_typed gamma f)
+    (Hty2: formula_typed gamma (elim_let_fmla f)),
+    formula_rep gamma_valid pd vt pf vv (elim_let_fmla f) Hty2 =
+    formula_rep gamma_valid pd vt pf vv f Hty1.
+Proof.
+  apply (elim_let_tm_fmla_rep (Right f) bt bf eq_refl eq_refl);
+  auto.
+Qed.
+
+End Rep.
+
+End ElimLetWhy3.
+
+(*Define the transformation*)
+Definition eliminate_let_term2 (gamma: context) : trans gamma :=
+  trans_goal gamma (elim_let_fmla true false).
+  
+Definition eliminate_let_fmla2 (gamma: context) : trans gamma :=
+  trans_goal gamma (elim_let_fmla false true).
+
+Definition eliminate_let2 (gamma: context) : trans gamma :=
+  trans_goal gamma (elim_let_fmla true true).
+
+(*Now we prove soundness*)
+Lemma eliminate_let_sound_gen2 (gamma: context) :
+  forall b1 b2,
+  sound_trans (trans_goal gamma (elim_let_fmla b1 b2)).
+Proof.
+  intros.
+  apply trans_goal_sound.
+  intros. split_all.
+  - apply elim_let_fmla_typed; auto.
+  - apply elim_let_fmla_fv.
+  - intros. erewrite elim_let_fmla_rep in H.
+    apply H.
+Qed.
+
+Theorem eliminate_let_term_sound2 gamma:
+  sound_trans (eliminate_let_term2 gamma).
+Proof.
+  apply eliminate_let_sound_gen2.
+Qed.
+
+Theorem eliminate_let_fmla_sound2 gamma:
+  sound_trans (eliminate_let_fmla2 gamma).
+Proof.
+  apply eliminate_let_sound_gen2.
+Qed.
+
+Theorem elim_let_sound2 gamma:
+  sound_trans (eliminate_let2 gamma).
+Proof.
+  apply eliminate_let_sound_gen2.
+Qed.
